word_lib: import changes from afp-2024
Signed-off-by: Gerwin Klein <gerwin.klein@proofcraft.systems>

lib/Word_Lib/Singleton_Bit_Shifts.thy
@@ -11,31 +11,40 @@ theory Singleton_Bit_Shifts
 begin
 
 definition shiftl1 :: \<open>'a::len word \<Rightarrow> 'a word\<close>
-  where \<open>shiftl1 = push_bit 1\<close>
+  where shiftl1_eq_double: \<open>shiftl1 = times 2\<close>
 
 lemma bit_shiftl1_iff [bit_simps]:
   \<open>bit (shiftl1 w) n \<longleftrightarrow> 0 < n \<and> n < LENGTH('a) \<and> bit w (n - 1)\<close>
   for w :: \<open>'a::len word\<close>
-  by (simp only: shiftl1_def bit_push_bit_iff) auto
+  by (auto simp add: shiftl1_eq_double bit_simps)
 
 definition shiftr1 :: \<open>'a::len word \<Rightarrow> 'a word\<close>
-  where \<open>shiftr1 = drop_bit 1\<close>
+  where shiftr1_eq_half: \<open>shiftr1 w = w div 2\<close>
 
 lemma bit_shiftr1_iff [bit_simps]:
   \<open>bit (shiftr1 w) n \<longleftrightarrow> bit w (Suc n)\<close>
   for w :: \<open>'a::len word\<close>
-  by (simp add: shiftr1_def bit_drop_bit_eq)
+  by (simp add: shiftr1_eq_half bit_Suc)
 
 definition sshiftr1 :: \<open>'a::len word \<Rightarrow> 'a word\<close>
-  where \<open>sshiftr1 \<equiv> signed_drop_bit 1\<close>
+  where sshiftr1_def: \<open>sshiftr1 = signed_drop_bit 1\<close>
 
 lemma bit_sshiftr1_iff [bit_simps]:
   \<open>bit (sshiftr1 w) n \<longleftrightarrow> bit w (if n = LENGTH('a) - 1 then LENGTH('a) - 1 else Suc n)\<close>
   for w :: \<open>'a::len word\<close>
-  by (auto simp add: sshiftr1_def bit_signed_drop_bit_iff)
+  by (auto simp add: sshiftr1_def bit_simps)
 
-lemma shiftr1_1: "shiftr1 (1::'a::len word) = 0"
-  by (simp add: shiftr1_def)
+lemma shiftl1_def:
+  \<open>shiftl1 = push_bit 1\<close>
+  by (rule ext, rule bit_word_eqI) (simp add: bit_simps mult.commute [of _ 2])
+
+lemma shiftr1_def:
+  \<open>shiftr1 = drop_bit 1\<close>
+  by (rule ext, rule bit_word_eqI) (simp add: bit_simps)
+
+lemma shiftr1_1:
+  \<open>shiftr1 (1::'a::len word) = 0\<close>
+  by (rule bit_word_eqI) (simp add: bit_simps)
 
 lemma sshiftr1_eq:
   \<open>sshiftr1 w = word_of_int (sint w div 2)\<close>
@@ -50,105 +59,108 @@ lemma shiftr1_eq:
   by (rule bit_word_eqI) (simp add: bit_simps flip: bit_Suc)
 
 lemma shiftl1_rev:
-  "shiftl1 w = word_reverse (shiftr1 (word_reverse w))"
+  \<open>shiftl1 w = word_reverse (shiftr1 (word_reverse w))\<close>
   by (rule bit_word_eqI) (auto simp add: bit_simps Suc_diff_Suc simp flip: bit_Suc)
 
 lemma shiftl1_p:
-  "shiftl1 w = w + w"
-  for w :: "'a::len word"
-  by (simp add: shiftl1_def)
+  \<open>shiftl1 w = w + w\<close>
+  by (rule bit_word_eqI) (simp add: bit_simps)
 
 lemma shiftr1_bintr:
-  "(shiftr1 (numeral w) :: 'a::len word) =
-    word_of_int (take_bit LENGTH('a) (numeral w) div 2)"
-  by (rule bit_word_eqI) (simp add: bit_simps bit_numeral_iff [where ?'a = int] flip: bit_Suc)
+  \<open>(shiftr1 (numeral w) :: 'a::len word) =
+    word_of_int (take_bit LENGTH('a) (numeral w) div 2)\<close>
+  apply (rule bit_word_eqI)
+  apply (simp add: bit_simps flip: bit_Suc)
+  done
 
 lemma sshiftr1_sbintr:
-  "(sshiftr1 (numeral w) :: 'a::len word) =
-    word_of_int (signed_take_bit (LENGTH('a) - 1) (numeral w) div 2)"
-  apply (cases \<open>LENGTH('a)\<close>)
-  apply simp_all
+  \<open>(sshiftr1 (numeral w) :: 'a::len word) =
+    word_of_int (signed_take_bit (LENGTH('a) - 1) (numeral w) div 2)\<close>
   apply (rule bit_word_eqI)
-  apply (auto simp add: bit_simps min_def simp flip: bit_Suc elim: le_SucE)
+  apply (simp add: bit_simps flip: bit_Suc)
+  apply transfer
+  apply auto
   done
 
 lemma shiftl1_wi:
-  "shiftl1 (word_of_int w) = word_of_int (2 * w)"
-  by (rule bit_word_eqI) (auto simp add: bit_simps)
+  \<open>shiftl1 (word_of_int w) = word_of_int (2 * w)\<close>
+  by (rule bit_word_eqI) (simp add: bit_simps)
 
 lemma shiftl1_numeral:
-  "shiftl1 (numeral w) = numeral (Num.Bit0 w)"
-  unfolding word_numeral_alt shiftl1_wi by simp
+  \<open>shiftl1 (numeral w) = numeral (Num.Bit0 w)\<close>
+  by (rule bit_word_eqI) (auto simp add: bit_simps bit_numeral_Bit0_iff)
 
 lemma shiftl1_neg_numeral:
-  "shiftl1 (- numeral w) = - numeral (Num.Bit0 w)"
-  unfolding word_neg_numeral_alt shiftl1_wi by simp
+  \<open>shiftl1 (- numeral w) = - numeral (Num.Bit0 w)\<close>
+  by (simp add: shiftl1_eq_double)
 
 lemma shiftl1_0:
-  "shiftl1 0 = 0"
-  by (simp add: shiftl1_def)
+  \<open>shiftl1 0 = 0\<close>
+  by (rule bit_word_eqI) (simp add: bit_simps)
 
 lemma shiftl1_def_u:
-  "shiftl1 w = word_of_int (2 * uint w)"
-  by (fact shiftl1_eq)
+  \<open>shiftl1 w = word_of_int (2 * uint w)\<close>
+  by (rule bit_word_eqI) (simp add: bit_simps)
 
 lemma shiftl1_def_s:
-  "shiftl1 w = word_of_int (2 * sint w)"
-  by (simp add: shiftl1_def)
+  \<open>shiftl1 w = word_of_int (2 * sint w)\<close>
+  by (rule bit_word_eqI) (simp add: bit_simps)
 
 lemma shiftr1_0:
-  "shiftr1 0 = 0"
-  by (simp add: shiftr1_def)
+  \<open>shiftr1 0 = 0\<close>
+  by (rule bit_word_eqI) (simp add: bit_simps)
 
 lemma sshiftr1_0:
-  "sshiftr1 0 = 0"
-  by (simp add: sshiftr1_def)
+  \<open>sshiftr1 0 = 0\<close>
+  by (rule bit_word_eqI) (simp add: bit_simps)
 
 lemma sshiftr1_n1:
-  "sshiftr1 (- 1) = - 1"
-  by (simp add: sshiftr1_def)
+  \<open>sshiftr1 (- 1) = - 1\<close>
+  by (rule bit_word_eqI) (auto simp add: bit_simps)
 
 lemma uint_shiftr1:
-  "uint (shiftr1 w) = uint w div 2"
+  \<open>uint (shiftr1 w) = uint w div 2\<close>
   by (rule bit_eqI) (simp add: bit_simps flip: bit_Suc)
 
 lemma shiftr1_div_2:
-  "uint (shiftr1 w) = uint w div 2"
+  \<open>uint (shiftr1 w) = uint w div 2\<close>
   by (fact uint_shiftr1)
 
 lemma sshiftr1_div_2:
-  "sint (sshiftr1 w) = sint w div 2"
-  by (rule bit_eqI) (auto simp add: bit_simps ac_simps min_def simp flip: bit_Suc elim: le_SucE)
+  \<open>sint (sshiftr1 w) = sint w div 2\<close>
+  by (rule bit_eqI) (auto simp add: bit_simps simp flip: bit_Suc)
 
 lemma nth_shiftl1:
-  "bit (shiftl1 w) n \<longleftrightarrow> n < size w \<and> n > 0 \<and> bit w (n - 1)"
+  \<open>bit (shiftl1 w) n \<longleftrightarrow> n < size w \<and> n > 0 \<and> bit w (n - 1)\<close>
   by (auto simp add: word_size bit_simps)
 
 lemma nth_shiftr1:
-  "bit (shiftr1 w) n = bit w (Suc n)"
+  \<open>bit (shiftr1 w) n = bit w (Suc n)\<close>
   by (fact bit_shiftr1_iff)
 
-lemma nth_sshiftr1: "bit (sshiftr1 w) n = (if n = size w - 1 then bit w n else bit w (Suc n))"
+lemma nth_sshiftr1:
+  \<open>bit (sshiftr1 w) n = (if n = size w - 1 then bit w n else bit w (Suc n))\<close>
   by (auto simp add: word_size bit_simps)
 
 lemma shiftl_power:
-  "(shiftl1 ^^ x) (y::'a::len word) = 2 ^ x * y"
-  by (induction x) (simp_all add: shiftl1_def)
+  \<open>(shiftl1 ^^ x) (y::'a::len word) = 2 ^ x * y\<close>
+  by (simp add: shiftl1_eq_double funpow_double_eq_push_bit push_bit_eq_mult)
 
 lemma le_shiftr1:
   \<open>shiftr1 u \<le> shiftr1 v\<close> if \<open>u \<le> v\<close>
-  using that by (simp add: word_le_nat_alt unat_div div_le_mono shiftr1_def drop_bit_Suc)
+  using that by (simp add: shiftr1_eq_half word_less_eq_imp_half_less_eq)
 
 lemma le_shiftr1':
-  "\<lbrakk> shiftr1 u \<le> shiftr1 v ; shiftr1 u \<noteq> shiftr1 v \<rbrakk> \<Longrightarrow> u \<le> v"
-  by (meson dual_order.antisym le_cases le_shiftr1)
+  \<open>u \<le> v\<close> if \<open>shiftr1 u \<le> shiftr1 v\<close> \<open>shiftr1 u \<noteq> shiftr1 v\<close>
+  by (rule word_half_less_imp_less_eq) (use that in \<open>simp add: shiftr1_eq_half\<close>)
 
 lemma sshiftr_eq_funpow_sshiftr1:
   \<open>w >>> n = (sshiftr1 ^^ n) w\<close>
-  apply (rule sym)
-  apply (simp add: sshiftr1_def sshiftr_def)
-  apply (induction n)
-   apply simp_all
-  done
+proof -
+  have \<open>sshiftr1 ^^ n = (signed_drop_bit n :: 'a word \<Rightarrow> _)\<close>
+    by (induction n) (simp_all add: sshiftr1_def)
+  then show ?thesis
+    by (simp add: sshiftr_def)
+qed
 
 end
