lib/Word_Lib/More_Word.thy
@@ -826,7 +826,7 @@ lemma word_2p_mult_inc:
   assumes x: "2 * 2 ^ n < (2::'a::len word) * 2 ^ m"
   assumes suc_n: "Suc n < LENGTH('a::len)"
   shows "2^n < (2::'a::len word)^m"
-  by (smt suc_n le_less_trans lessI nat_less_le nat_mult_less_cancel_disj p2_gt_0
+  by (smt (verit) suc_n le_less_trans lessI nat_less_le nat_mult_less_cancel_disj p2_gt_0
           power_Suc power_Suc unat_power_lower word_less_nat_alt x)
 
 lemma power_overflow:
@@ -1198,7 +1198,7 @@ lemma unat_Suc2:
 
 lemma word_div_1:
   "(n :: 'a :: len word) div 1 = n"
-  by (fact bits_div_by_1)
+  by (fact div_by_1)
 
 lemma word_minus_one_le:
   "-1 \<le> (x :: 'a :: len word) = (x = -1)"
@@ -2094,7 +2094,7 @@ lemma degenerate_word:"LENGTH('a) = 1 \<Longrightarrow> (x::('a::len) word) = 0 
   by (metis One_nat_def less_irrefl_nat sint_1_cases)
 
 lemma div_by_0_word: "(x::'a::len word) div 0 = 0"
-  by (fact bits_div_by_0)
+  by (fact div_by_0)
 
 lemma div_less_dividend_word:"\<lbrakk>x \<noteq> 0; n \<noteq> 1\<rbrakk> \<Longrightarrow> (x::('a::len) word) div n < x"
   apply (cases \<open>n = 0\<close>)
@@ -2232,8 +2232,7 @@ lemma word_ops_nth:
 lemma word_power_nonzero:
   "\<lbrakk> (x :: 'a::len word) < 2 ^ (LENGTH('a) - n); n < LENGTH('a); x \<noteq> 0 \<rbrakk>
   \<Longrightarrow> x * 2 ^ n \<noteq> 0"
-  by (metis Word.word_div_mult bits_div_0 len_gt_0 len_of_finite_2_def nat_mult_power_less_eq
-    p2_gt_0 unat_mono unat_power_lower word_gt_a_gt_0)
+  by (metis gr0I mult.commute not_less_eq p2_gt_0 power_0 word_less_1 word_power_less_diff zero_less_diff)
 
 lemma less_1_helper:
   "n \<le> m \<Longrightarrow> (n - 1 :: int) < m"
@@ -2411,7 +2410,7 @@ lemma eq_ucast_ucast_eq:
 lemma le_ucast_ucast_le:
   "x \<le> ucast y \<Longrightarrow> ucast x \<le> y"
   for x :: "'a::len word" and y :: "'b::len word"
-  by (smt le_unat_uoi linorder_not_less order_less_imp_le ucast_nat_def unat_arith_simps(1))
+  by (smt (verit) le_unat_uoi linorder_not_less order_less_imp_le ucast_nat_def unat_arith_simps(1))
 
 lemma less_ucast_ucast_less:
   "LENGTH('b) \<le> LENGTH('a) \<Longrightarrow> x < ucast y \<Longrightarrow> ucast x < y"
